YulEvmCompiler/SsaCfg/Implementation/OfYulSound.lean
@@ -9,7 +9,11 @@ import YulEvmCompiler.SsaCfg.Implementation.OfYulSound.CurInduction
 import YulEvmCompiler.SsaCfg.Implementation.OfYulSound.NoShadow
 import YulEvmCompiler.SsaCfg.Implementation.OfYulSound.Loop
 import YulEvmCompiler.SsaCfg.Implementation.OfYulSound.LoopSim
+import YulEvmCompiler.SsaCfg.Implementation.OfYulSound.LoopStepSim
 import YulEvmCompiler.SsaCfg.Implementation.OfYulSound.Switch
+import YulEvmCompiler.SsaCfg.Implementation.OfYulSound.CallSim
+import YulEvmCompiler.SsaCfg.Implementation.OfYulSound.CondSim
+import YulEvmCompiler.SsaCfg.Implementation.OfYulSound.BlockSim
 import YulEvmCompiler.SsaCfg.Implementation.OfYulSound.Sim
 set_option warningAsError true
 /-!
